Translation/Global.lean
@@ -19,22 +19,24 @@ def Surface.is_valid_ctor_ty (G : Surface.GlobalEnv) : Surface.Ty -> Option Stri
           if Surface.is_data G x then return x else none
 
 
-def Surface.Ty.translate_ctors (G : Core.GlobalEnv) (ctors : Vect n  (String × Surface.Ty)) : Option (Vect n (String × Core.Ty)) := do
-  -- check that names are unique
-  let cns : Vect n String := (λ x => x.1) <$> ctors
+def Surface.Ty.translate_ctors (ctors : Vect n (String × Surface.Ty)) : (Vect n (String × Core.Ty)) :=
+  (λ (x, ty) => (x , ty.translate)) <$> ctors
 
-  let octors : Vect n (Option (String × Core.Ty)) :=  (λ (x, ty) =>
-    do let ty' := ty.translate
-       let _ <- Core.is_valid_ctor_ty G ty'
-       return (x , ty')) <$> ctors
-  octors.seq
+def Core.Ty.check_ctor_tys (dx : String) (G : Core.GlobalEnv) (ctors : Vect n (String × Core.Ty)) : Option Unit := do
+  let check : Vect n (Option String) :=
+      (λ c => Core.is_valid_ctor_ty  G c.2) <$> ctors
+  let check' <- check.seq
+  -- TODO: check that names are unique
+  -- let cns : Vect n String := (λ x => x.1) <$> ctors
+  if check'.elems_eq_to dx then return () else none
 
 
 
 @[simp]
 def Surface.Global.translate (G : Core.GlobalEnv) : Global -> Option Core.Global
 | .data (n := n) x K ctors => do
-  let ctors' <- Ty.translate_ctors ((Core.Global.data 0 x K.translate Vect.nil) :: G) ctors
+  let ctors' := Ty.translate_ctors ctors
+  Core.Ty.check_ctor_tys x (.data 0 x K.translate Vect.nil :: G) ctors'
   return Core.Global.data n x K.translate ctors'
 
 @[simp]
@@ -44,7 +46,6 @@ def Surface.GlobalEnv.translate : Surface.GlobalEnv -> Option (Core.GlobalEnv)
   let gs' <- Surface.GlobalEnv.translate gs
   let g' <- g.translate gs'
   return g' :: gs'
-
 
 namespace Test.Core.Global
 
